fixing bug #154. This was an ugly one ... thankfully, nothingin the regression suite depended on the bug, but, if you're counting on some example that is not in the suite, then PLEASE REVERIFY YOUR CODE!'

src/tc/tc.fs
@@ -365,7 +365,7 @@ and tc_typ env (t:typ) : typ * knd * guard_t =
                       then Util.fprint3 "Checking argument %s against expected kind %s\n>>>Got guard %s\n"
                              (Print.arg_to_string actual) (Print.kind_to_string formal_k) (Rel.guard_to_string env g');
                       let actual = Inl t, imp in
-                      let g' = Rel.imp_guard (Rel.guard_of_guard_formula <| Tc.Util.short_circuit_guard (Inl head) outargs) g' in
+                      let g' = Rel.imp_guard (Rel.guard_of_guard_formula <| Tc.Util.short_circuit_typ (Inl head) outargs) g' in
                       let subst = maybe_extend_subst subst formal actual in
                       check_explicit_args (actual::outargs) subst (Rel.conj_guard g g') formals actuals
 
@@ -376,7 +376,7 @@ and tc_typ env (t:typ) : typ * knd * guard_t =
                       if Env.debug env Options.High then Util.fprint2 "Checking argument %s against expected type %s\n" (Print.arg_to_string actual) (Print.typ_to_string tx);
                       let v, _, g' = tc_total_exp env' v in
                       let actual = Inr v, imp in
-                      let g' = Rel.imp_guard (Rel.guard_of_guard_formula <| Tc.Util.short_circuit_guard (Inl head) outargs) g' in
+                      let g' = Rel.imp_guard (Rel.guard_of_guard_formula <| Tc.Util.short_circuit_typ (Inl head) outargs) g' in
                       let subst = maybe_extend_subst subst formal actual in
                       check_explicit_args (actual::outargs) subst (Rel.conj_guard g g') formals actuals
 
@@ -755,177 +755,199 @@ and tc_exp env e : exp * lcomp * guard_t =
     let env = Tc.Env.clear_expected_typ env |> fst |> instantiate_both in 
     if debug env Options.High then Util.fprint2 "(%s) Checking app %s\n" (Range.string_of_range top.pos) (Print.exp_to_string top);
     let head, chead, g_head = tc_exp (no_inst env) head in //Don't instantiate f; instantiations will be computed below, accounting for implicits/explicits
-    let thead = chead.res_typ in
-    if debug env Options.High then Util.fprint2 "(%s) Type of head is %s\n" (Range.string_of_range head.pos) (Print.typ_to_string thead);
-    let rec check_function_app norm tf = match (Util.unrefine tf).n with 
-        | Typ_uvar _
-        | Typ_app({n=Typ_uvar _}, _) ->
-          let rec tc_args env args : (Syntax.args * list<lcomp> * guard_t) = match args with
-                | [] -> ([], [], Rel.trivial_guard)
-                | (Inl t, _)::_ -> 
-                  raise (Error("Explicit type applications on a term with unknown type; add an annotation?", t.pos))
-                | (Inr e, imp)::tl -> 
-                  let e, c, g_e = tc_exp env e in 
-                  let args, comps, g_rest = tc_args env tl in 
-                  (Inr e, imp)::args, c::comps, Rel.conj_guard g_e g_rest in
-          (* Infer: t1 -> ... -> tn -> ML ('u x1...xm), 
-                    where ti are the result types of each arg
-                    and   xi are the free type/term variables in the environment *)
-          let args, comps, g_args = tc_args env args in 
-          let bs = null_binders_of_tks (Tc.Util.tks_of_args args) in
-          let cres = Util.ml_comp (Tc.Util.new_tvar env ktype) top.pos in
-          Tc.Util.force_trivial env <| Rel.teq env tf (mk_Typ_fun(bs, cres) (Some ktype) tf.pos);
-          let comp = List.fold_right (fun c out -> Tc.Util.bind env None c (None, out)) (chead::comps) (Tc.Util.lcomp_of_comp <| cres) in
-          mk_Exp_app(head, args) (Some comp.res_typ) top.pos, comp, Rel.conj_guard g_head g_args
-
-        | Typ_fun(bs, c) -> 
-          let vars = Tc.Env.binders env in
-          
-          let rec tc_args (subst,   (* substituting actuals for formals seen so far, when actual is pure *)
-                           outargs, (* type-checked actuals *)
-                           arg_rets,(* The results of each argument at the logic level *)
-                           comps,   (* computation types for each actual *)
-                           g,       (* conjoined guard formula for all the actuals *)
-                           fvs)     (* unsubstituted formals, to check that they do not occur free elsewhere in the type of f *)
-                           bs       (* formal parameters *)
-                           (cres:lcomp)     (* function result comp *)
-                           args     (* actual arguments  *) : (exp * lcomp * guard_t) =
-           match bs, args with 
-            | (Inl a, _)::rest, (Inr e, _)::_ -> (* instantiate a type argument *) 
-              let k = Util.subst_kind subst a.sort in
-              fxv_check head env (Inl k) fvs;
-              let targ = 
-              
-              fst <| Tc.Rel.new_tvar e.pos vars k in 
-              if debug env Options.Extreme then Util.fprint2 "Instantiating %s to %s" (Print.strBvd a.v) (Print.typ_to_string targ);
-              let subst = (Inl(a.v, targ))::subst in
-              let arg = Inl targ, as_implicit true in
-              tc_args (subst, arg::outargs, arg::arg_rets, comps, g, fvs) rest cres args
-
-            | (Inr x, Some Implicit)::rest, (_, None)::_ -> (* instantiate an implicit value arg *)
-              let t = Util.subst_typ subst x.sort in
-              fxv_check head env (Inr t) fvs;
-              let varg = Tc.Util.new_evar env t in
-              let subst = (Inr(x.v, varg))::subst in
-              let arg = Inr varg, as_implicit true in
-              tc_args (subst, arg::outargs, arg::arg_rets, comps, g, fvs) rest cres args
-
-            | (Inl a, aqual)::rest, (Inl t, _)::rest' -> (* a concrete type argument *)
-              if debug env Options.Extreme then Util.fprint2 "\tGot a type arg for %s = %s\n" (Print.strBvd a.v) (Print.typ_to_string t);
-              let k = Util.subst_kind subst a.sort in 
-              fxv_check head env (Inl k) fvs;
-              let t, g' = tc_typ_check ({env with use_eq=is_eq aqual}) t k in
-              let g' = Tc.Rel.imp_guard (Rel.guard_of_guard_formula <| Tc.Util.short_circuit_guard (Inr head) outargs) g' in
-              let f = Tc.Util.label_guard Errors.ill_kinded_type t.pos (guard_f g') in
-              let g' = {g' with Rel.guard_f=f} in
-              let arg = targ t in 
-              let subst = maybe_extend_subst subst (List.hd bs) arg in
-              tc_args (subst, arg::outargs, arg::arg_rets, comps, Rel.conj_guard g g', fvs) rest cres rest'
-
-            | (Inr x, aqual)::rest, (Inr e, _)::rest' -> (* a concrete exp argument *)
-              if debug env Options.Extreme then Util.fprint2 "\tType of arg (before subst (%s)) = %s\n" (Print.subst_to_string subst) (Print.typ_to_string x.sort);
-              let targ = Util.subst_typ subst x.sort in 
-              if debug env Options.Extreme then  Util.fprint1 "\tType of arg (after subst) = %s\n" (Print.typ_to_string targ);
-              fxv_check head env (Inr targ) fvs;
-              let env = Tc.Env.set_expected_typ env targ in
-              let env = {env with use_eq=is_eq aqual} in
-              if debug env <| Options.Other "EQ" && env.use_eq then Util.fprint2 "Checking arg %s at type %s with an equality constraint!\n" (Print.exp_to_string e) (Print.typ_to_string targ);
-              if debug env Options.High then  Util.fprint3 "Checking arg (%s) %s at type %s\n" (Print.tag_of_exp e) (Print.exp_to_string e) (Print.typ_to_string targ);
-              let e, c, g_e = tc_exp env e in 
-              let c = Tc.Util.weaken_precondition env c (Tc.Util.short_circuit_guard (Inr head) outargs) in
-              let g = Rel.conj_guard g g_e in
-              if debug env Options.High then Util.fprint2 "Guard on this arg is %s;\naccumulated guard is %s\n" (Rel.guard_to_string env g_e) (Rel.guard_to_string env g);
-              if Util.is_total_lcomp c 
-              then let arg = varg e in 
-                   let subst = maybe_extend_subst subst (List.hd bs) arg in
-                   tc_args (subst, arg::outargs, arg::arg_rets, comps, g, fvs) rest cres rest'
-              else if Tc.Util.is_pure_effect env c.eff_name 
-              then let arg = varg e in
-                   let subst = maybe_extend_subst subst (List.hd bs) arg in
-                   let comps, guard =
-                      (Some (Env.Binding_var(x.v, x.sort)), c)::comps, g in
-                   tc_args (subst, arg::outargs, arg::arg_rets, comps, guard, fvs) rest cres rest'
-              else if is_null_binder (List.hd bs)
-              then let newx = Util.gen_bvar_p e.pos c.res_typ in
-                   let arg = varg <| bvar_to_exp newx in
-                   let binding = Env.Binding_var(newx.v, newx.sort) in
-                   tc_args (subst, (varg e)::outargs, arg::arg_rets, (Some binding, c)::comps, g, fvs) rest cres rest'
-              else tc_args (subst, (varg e)::outargs, (varg <| bvar_to_exp x)::arg_rets, (Some <| Env.Binding_var(x.v, x.sort), c)::comps, g, Util.set_add x fvs) rest cres rest'
-
-            | _, [] -> (* full or partial application *) 
-              fxv_check head env (Inr cres.res_typ) fvs;
-              let cres, g = match bs with 
-                | [] -> (* full app *)
-                    let cres = Tc.Util.subst_lcomp subst cres in 
-                    (* If we have f e1 e2
-                       where e1 or e2 is impure but f is a pure function, 
-                       then refine the result to be equal to f x1 x2, 
-                       where xi is the result of ei. (See the last two tests in examples/unit-tests/unit1.fst)
-                    *)
-                    let g = Rel.conj_guard g_head g in
-
-                    let refine_with_equality = 
-                        //if the function is pure, but its arguments are not, then add an equality refinement here
-                        //OW, for pure applications we always add an equality at the end; see ADD_EQ_REFINEMENT below
-                        Util.is_pure_lcomp cres
-                        && comps |> Util.for_some (fun (_, c) -> not (Util.is_pure_lcomp c)) in (* if the guard is trivial, then strengthen_precondition below will not add an equality; so add it here *)
-                      
-                    let cres = //NS: Choosing when to add an equality refinement is VERY important for performance. Adding it unconditionally impacts run time by >5x
-                        if refine_with_equality 
-                        then Util.maybe_assume_result_eq_pure_term env (mk_Exp_app_flat(head, List.rev arg_rets) (Some cres.res_typ) top.pos) cres
-                        else (if Env.debug env Options.Low
-                              then Util.fprint3 "Not refining result: f=%s; cres=%s; guard=%s\n" (Print.exp_to_string head) (Print.lcomp_typ_to_string cres) (Rel.guard_to_string env g);
-                              cres) in
-
-                    (* relabeling the labeled sub-terms in cres to report failing pre-conditions at this call-site *)
-                    Tc.Util.refresh_comp_label env false cres, g
-                
-                | _ ->  (* partial app *)
-                  let g = Rel.conj_guard g_head g |> Rel.solve_deferred_constraints env in
-                  Tc.Util.lcomp_of_comp <| mk_Total  (Util.subst_typ subst <| mk_Typ_fun(bs, cres.comp()) (Some ktype) top.pos), g in
-            
-              if debug env Options.Low then Util.fprint1 "\t Type of result cres is %s\n" (Print.lcomp_typ_to_string cres);
-              let comp = List.fold_left (fun out c -> Tc.Util.bind env None (snd c) (fst c, out)) cres comps in
-              let comp = Tc.Util.bind env None chead (None, comp) in
-              let app =  mk_Exp_app_flat(head, List.rev outargs) (Some comp.res_typ) top.pos in
-              let comp, g = Tc.Util.strengthen_precondition None env app comp g in //Each conjunct in g is already labeled
-              if debug env Options.Low then Util.fprint2 "\t Type of app term %s is %s\n" (Normalize.exp_norm_to_string env app) (Print.lcomp_typ_to_string comp);
-              app, comp, g
-               
-            | (Inr _, _)::_, (Inl _, _)::_ ->
-              raise (Error(Util.format1 "Unexpected type argument (%s)" (Print.exp_to_string top), argpos (List.hd args)))
-
-            | [], arg::_ -> (* too many args, except maybe c returns a function *) 
-              let rec aux norm tres = 
-                let tres = Util.compress_typ tres |> Util.unrefine in 
-                match tres.n with 
-                    | Typ_fun(bs, cres') -> 
-                      if debug env Options.Low then Util.fprint1 "%s: Warning: Potentially redundant explicit currying of a function type \n" (Range.string_of_range tres.pos);
-                      tc_args (subst, outargs, arg_rets, (None, cres)::comps, g, fvs) bs (Tc.Util.lcomp_of_comp cres') args
-                    | _ when (not norm) ->
-                        aux true (whnf env tres)
-                    | _ -> raise (Error(Util.format2 "Too many arguments to function of type %s; got %s" (Normalize.typ_norm_to_string env tf) (Print.exp_to_string top), argpos arg)) in
-              aux false cres.res_typ in
-         
-          tc_args ([], [], [], [], Rel.trivial_guard, no_fvs.fxvs) bs (Tc.Util.lcomp_of_comp c) args
+    let aux () = 
+        let n_args = List.length args in
+        match head.n with 
+            | Exp_fvar(fv, _) when ((lid_equals fv.v Const.op_And || lid_equals fv.v Const.op_Or) && n_args = 2) -> //short-circuiting
+              let env = Tc.Env.set_expected_typ env t_bool in 
+              begin match args with 
+                | [(Inr e1, _); (Inr e2, _)] -> 
+                  let e1, c1, g1 = tc_exp env e1 in 
+                  let e2, c2, g2 = tc_exp env e2 in 
+                  let x = gen_bvar t_bool in 
+                  let xexp = bvar_to_exp x in
+                  let c2 = 
+                    if lid_equals fv.v Const.op_And
+                    then Tc.Util.ite env (Util.b2t <| bvar_to_exp x) c2 (Tc.Util.return_value env t_bool xexp |> Util.lcomp_of_comp)
+                    else Tc.Util.ite env (Util.b2t <| bvar_to_exp x) (Tc.Util.return_value env t_bool xexp |> Util.lcomp_of_comp) c2 in
+                  let c = Tc.Util.bind env None c1 (Some <| Tc.Env.Binding_var(x.v, t_bool), c2) in
+                  let e = mk_Exp_app(head, [varg e1; varg e2]) (Some t_bool) top.pos in
+                  e, c, Rel.conj_guard g_head (Rel.conj_guard g1 g2)
                   
-        | _ -> 
-            if not norm
-            then check_function_app true (whnf env tf) 
-            else raise (Error(Tc.Errors.expected_function_typ env tf, head.pos)) in
+                | _ -> raise (Error("Expected two boolean arguments", head.pos))  
+              end
+         
+            | _ ->  
+            let thead = chead.res_typ in
+            if debug env Options.High then Util.fprint2 "(%s) Type of head is %s\n" (Range.string_of_range head.pos) (Print.typ_to_string thead);
+            let rec check_function_app norm tf = match (Util.unrefine tf).n with 
+                | Typ_uvar _
+                | Typ_app({n=Typ_uvar _}, _) ->
+                  let rec tc_args env args : (Syntax.args * list<lcomp> * guard_t) = match args with
+                        | [] -> ([], [], Rel.trivial_guard)
+                        | (Inl t, _)::_ -> 
+                          raise (Error("Explicit type applications on a term with unknown type; add an annotation?", t.pos))
+                        | (Inr e, imp)::tl -> 
+                          let e, c, g_e = tc_exp env e in 
+                          let args, comps, g_rest = tc_args env tl in 
+                          (Inr e, imp)::args, c::comps, Rel.conj_guard g_e g_rest in
+                  (* Infer: t1 -> ... -> tn -> ML ('u x1...xm), 
+                            where ti are the result types of each arg
+                            and   xi are the free type/term variables in the environment *)
+                  let args, comps, g_args = tc_args env args in 
+                  let bs = null_binders_of_tks (Tc.Util.tks_of_args args) in
+                  let cres = Util.ml_comp (Tc.Util.new_tvar env ktype) top.pos in
+                  Tc.Util.force_trivial env <| Rel.teq env tf (mk_Typ_fun(bs, cres) (Some ktype) tf.pos);
+                  let comp = List.fold_right (fun c out -> Tc.Util.bind env None c (None, out)) (chead::comps) (Tc.Util.lcomp_of_comp <| cres) in
+                  mk_Exp_app(head, args) (Some comp.res_typ) top.pos, comp, Rel.conj_guard g_head g_args
 
-    let e, c, g = check_function_app false (Util.unrefine thead) in
-    let c = if !Options.verify 
-            && not (Util.is_lcomp_partial_return c)
-            && Util.is_pure_lcomp c //ADD_EQ_REFINEMENT for pure applications
-            then Tc.Util.maybe_assume_result_eq_pure_term env e c 
-            else c in
-    if debug env Options.Extreme 
-    then Util.fprint3 "(%s) About to check %s against expected typ %s\n" (Range.string_of_range e.pos) 
-          (Print.typ_to_string c.res_typ)
-          (Env.expected_typ env0 |> (fun x -> match x with None -> "None" | Some t -> Print.typ_to_string t));
-    let e, c, g' = comp_check_expected_typ env0 e c in
-    e, c, Rel.conj_guard g g'
+                | Typ_fun(bs, c) -> 
+                  let vars = Tc.Env.binders env in
+          
+                  let rec tc_args (subst,   (* substituting actuals for formals seen so far, when actual is pure *)
+                                   outargs, (* type-checked actuals *)
+                                   arg_rets,(* The results of each argument at the logic level *)
+                                   comps,   (* computation types for each actual *)
+                                   g,       (* conjoined guard formula for all the actuals *)
+                                   fvs)     (* unsubstituted formals, to check that they do not occur free elsewhere in the type of f *)
+                                   bs       (* formal parameters *)
+                                   (cres:lcomp)     (* function result comp *)
+                                   args     (* actual arguments  *) : (exp * lcomp * guard_t) =
+                   match bs, args with 
+                    | (Inl a, _)::rest, (Inr e, _)::_ -> (* instantiate a type argument *) 
+                      let k = Util.subst_kind subst a.sort in
+                      fxv_check head env (Inl k) fvs;
+                      let targ = 
+              
+                      fst <| Tc.Rel.new_tvar e.pos vars k in 
+                      if debug env Options.Extreme then Util.fprint2 "Instantiating %s to %s" (Print.strBvd a.v) (Print.typ_to_string targ);
+                      let subst = (Inl(a.v, targ))::subst in
+                      let arg = Inl targ, as_implicit true in
+                      tc_args (subst, arg::outargs, arg::arg_rets, comps, g, fvs) rest cres args
+
+                    | (Inr x, Some Implicit)::rest, (_, None)::_ -> (* instantiate an implicit value arg *)
+                      let t = Util.subst_typ subst x.sort in
+                      fxv_check head env (Inr t) fvs;
+                      let varg = Tc.Util.new_evar env t in
+                      let subst = (Inr(x.v, varg))::subst in
+                      let arg = Inr varg, as_implicit true in
+                      tc_args (subst, arg::outargs, arg::arg_rets, comps, g, fvs) rest cres args
+
+                    | (Inl a, aqual)::rest, (Inl t, _)::rest' -> (* a concrete type argument *)
+                      if debug env Options.Extreme then Util.fprint2 "\tGot a type arg for %s = %s\n" (Print.strBvd a.v) (Print.typ_to_string t);
+                      let k = Util.subst_kind subst a.sort in 
+                      fxv_check head env (Inl k) fvs;
+                      let t, g' = tc_typ_check ({env with use_eq=is_eq aqual}) t k in
+                      let f = Tc.Util.label_guard Errors.ill_kinded_type t.pos (guard_f g') in
+                      let g' = {g' with Rel.guard_f=f} in
+                      let arg = targ t in 
+                      let subst = maybe_extend_subst subst (List.hd bs) arg in
+                      tc_args (subst, arg::outargs, arg::arg_rets, comps, Rel.conj_guard g g', fvs) rest cres rest'
+
+                    | (Inr x, aqual)::rest, (Inr e, _)::rest' -> (* a concrete exp argument *)
+                      if debug env Options.Extreme then Util.fprint2 "\tType of arg (before subst (%s)) = %s\n" (Print.subst_to_string subst) (Print.typ_to_string x.sort);
+                      let targ = Util.subst_typ subst x.sort in 
+                      if debug env Options.Extreme then  Util.fprint1 "\tType of arg (after subst) = %s\n" (Print.typ_to_string targ);
+                      fxv_check head env (Inr targ) fvs;
+                      let env = Tc.Env.set_expected_typ env targ in
+                      let env = {env with use_eq=is_eq aqual} in
+                      if debug env <| Options.Other "EQ" && env.use_eq then Util.fprint2 "Checking arg %s at type %s with an equality constraint!\n" (Print.exp_to_string e) (Print.typ_to_string targ);
+                      if debug env Options.High then  Util.fprint3 "Checking arg (%s) %s at type %s\n" (Print.tag_of_exp e) (Print.exp_to_string e) (Print.typ_to_string targ);
+                      let e, c, g_e = tc_exp env e in 
+                      let g = Rel.conj_guard g g_e in
+                      if debug env Options.High then Util.fprint2 "Guard on this arg is %s;\naccumulated guard is %s\n" (Rel.guard_to_string env g_e) (Rel.guard_to_string env g);
+                      if Util.is_total_lcomp c 
+                      then let arg = varg e in 
+                           let subst = maybe_extend_subst subst (List.hd bs) arg in
+                           tc_args (subst, arg::outargs, arg::arg_rets, comps, g, fvs) rest cres rest'
+                      else if Tc.Util.is_pure_effect env c.eff_name 
+                      then let arg = varg e in
+                           let subst = maybe_extend_subst subst (List.hd bs) arg in
+                           let comps, guard =
+                              (Some (Env.Binding_var(x.v, x.sort)), c)::comps, g in
+                           tc_args (subst, arg::outargs, arg::arg_rets, comps, guard, fvs) rest cres rest'
+                      else if is_null_binder (List.hd bs)
+                      then let newx = Util.gen_bvar_p e.pos c.res_typ in
+                           let arg = varg <| bvar_to_exp newx in
+                           let binding = Env.Binding_var(newx.v, newx.sort) in
+                           tc_args (subst, (varg e)::outargs, arg::arg_rets, (Some binding, c)::comps, g, fvs) rest cres rest'
+                      else tc_args (subst, (varg e)::outargs, (varg <| bvar_to_exp x)::arg_rets, (Some <| Env.Binding_var(x.v, x.sort), c)::comps, g, Util.set_add x fvs) rest cres rest'
+
+                    | _, [] -> (* full or partial application *) 
+                      fxv_check head env (Inr cres.res_typ) fvs;
+                      let cres, g = match bs with 
+                        | [] -> (* full app *)
+                            let cres = Tc.Util.subst_lcomp subst cres in 
+                            (* If we have f e1 e2
+                               where e1 or e2 is impure but f is a pure function, 
+                               then refine the result to be equal to f x1 x2, 
+                               where xi is the result of ei. (See the last two tests in examples/unit-tests/unit1.fst)
+                            *)
+                            let g = Rel.conj_guard g_head g in
+
+                            let refine_with_equality = 
+                                //if the function is pure, but its arguments are not, then add an equality refinement here
+                                //OW, for pure applications we always add an equality at the end; see ADD_EQ_REFINEMENT below
+                                Util.is_pure_lcomp cres
+                                && comps |> Util.for_some (fun (_, c) -> not (Util.is_pure_lcomp c)) in (* if the guard is trivial, then strengthen_precondition below will not add an equality; so add it here *)
+                      
+                            let cres = //NS: Choosing when to add an equality refinement is VERY important for performance. Adding it unconditionally impacts run time by >5x
+                                if refine_with_equality 
+                                then Util.maybe_assume_result_eq_pure_term env (mk_Exp_app_flat(head, List.rev arg_rets) (Some cres.res_typ) top.pos) cres
+                                else (if Env.debug env Options.Low
+                                      then Util.fprint3 "Not refining result: f=%s; cres=%s; guard=%s\n" (Print.exp_to_string head) (Print.lcomp_typ_to_string cres) (Rel.guard_to_string env g);
+                                      cres) in
+
+                            (* relabeling the labeled sub-terms in cres to report failing pre-conditions at this call-site *)
+                            Tc.Util.refresh_comp_label env false cres, g
+                
+                        | _ ->  (* partial app *)
+                          let g = Rel.conj_guard g_head g |> Rel.solve_deferred_constraints env in
+                          Tc.Util.lcomp_of_comp <| mk_Total  (Util.subst_typ subst <| mk_Typ_fun(bs, cres.comp()) (Some ktype) top.pos), g in
+            
+                      if debug env Options.Low then Util.fprint1 "\t Type of result cres is %s\n" (Print.lcomp_typ_to_string cres);
+                      let comp = List.fold_left (fun out c -> Tc.Util.bind env None (snd c) (fst c, out)) cres comps in
+                      let comp = Tc.Util.bind env None chead (None, comp) in
+                      let app =  mk_Exp_app_flat(head, List.rev outargs) (Some comp.res_typ) top.pos in
+                      let comp, g = Tc.Util.strengthen_precondition None env app comp g in //Each conjunct in g is already labeled
+                      if debug env Options.Low then Util.fprint2 "\t Type of app term %s is %s\n" (Normalize.exp_norm_to_string env app) (Print.lcomp_typ_to_string comp);
+                      app, comp, g
+               
+                    | (Inr _, _)::_, (Inl _, _)::_ ->
+                      raise (Error(Util.format1 "Unexpected type argument (%s)" (Print.exp_to_string top), argpos (List.hd args)))
+
+                    | [], arg::_ -> (* too many args, except maybe c returns a function *) 
+                      let rec aux norm tres = 
+                        let tres = Util.compress_typ tres |> Util.unrefine in 
+                        match tres.n with 
+                            | Typ_fun(bs, cres') -> 
+                              if debug env Options.Low then Util.fprint1 "%s: Warning: Potentially redundant explicit currying of a function type \n" (Range.string_of_range tres.pos);
+                              tc_args (subst, outargs, arg_rets, (None, cres)::comps, g, fvs) bs (Tc.Util.lcomp_of_comp cres') args
+                            | _ when (not norm) ->
+                                aux true (whnf env tres)
+                            | _ -> raise (Error(Util.format2 "Too many arguments to function of type %s; got %s" (Normalize.typ_norm_to_string env tf) (Print.exp_to_string top), argpos arg)) in
+                      aux false cres.res_typ in
+         
+                  tc_args ([], [], [], [], Rel.trivial_guard, no_fvs.fxvs) bs (Tc.Util.lcomp_of_comp c) args
+                  
+                | _ -> 
+                    if not norm
+                    then check_function_app true (whnf env tf) 
+                    else raise (Error(Tc.Errors.expected_function_typ env tf, head.pos)) in
+            check_function_app false (Util.unrefine thead) in
+
+        let e, c, g = aux () in
+        let c = if !Options.verify 
+                && not (Util.is_lcomp_partial_return c)
+                && Util.is_pure_lcomp c //ADD_EQ_REFINEMENT for pure applications
+                then Tc.Util.maybe_assume_result_eq_pure_term env e c 
+                else c in
+        if debug env Options.Extreme 
+        then Util.fprint3 "(%s) About to check %s against expected typ %s\n" (Range.string_of_range e.pos) 
+              (Print.typ_to_string c.res_typ)
+              (Env.expected_typ env0 |> (fun x -> match x with None -> "None" | Some t -> Print.typ_to_string t));
+        let e, c, g' = comp_check_expected_typ env0 e c in
+        e, c, Rel.conj_guard g g'
           
   | Exp_match(e1, eqns) -> 
     let env1, topt = Env.clear_expected_typ env in 
