examples/bug-reports/bug154c.fst
@@ -1,4 +1,4 @@
 module Bug154c
 
-val ff : u:unit -> Lemma (False)
-let ff u = ignore (false && 1 = 2)
+val ff : unit -> Lemma (ensures False)
+let ff u = ignore (false && (0 = 1))
